Generalize mpred to support more logics

theories/lang/cpp/logic/mpred.v
@@ -4,13 +4,15 @@
  * See the LICENSE-BedRock file in the repository root for details.
  *)
 (**
-This file defines the core [bi] (called [mpred]) that we use for C++.
-The core logic is defined in [pred.v]. *)
+This file axiomatizes and instantiates [mpred] with the ghost types of the logic
+that we use for C++.
+The core C++ logic is defined in [pred.v]. *)
 From iris.base_logic.lib Require Import own cancelable_invariants.
 Require Import iris.bi.monpred.
 
 From bedrock.prelude Require Import base.
 From bedrock.lang Require Import bi.prelude.
+Require Export bedrock.lang.base_logic.mpred.
 Import ChargeNotation.
 
 Module Type CPP_LOGIC_CLASS_BASE.
@@ -18,80 +20,44 @@ Module Type CPP_LOGIC_CLASS_BASE.
   Axiom has_inv : forall Σ, cppG Σ -> invGS Σ.
   Axiom has_cinv : forall Σ, cppG Σ -> cinvG Σ.
 
-  #[global] Existing Instances has_inv has_cinv.
-
-  Existing Class cppG.
-
   Parameter _cpp_ghost : Type.
 End CPP_LOGIC_CLASS_BASE.
 
 Module Type CPP_LOGIC_CLASS_MIXIN (Import CC : CPP_LOGIC_CLASS_BASE).
+
+  Definition cpp_preGS Σ thread_info : LOGIC.GpreS Σ thread_info := {|
+    LOGIC.preGS := cppG Σ
+  ; LOGIC.preGS_has_inv := has_inv Σ
+  ; LOGIC.preGS_has_cinv := has_cinv Σ
+  |}.
+  Definition cpp_GS Σ thread_info : LOGIC.GS Σ thread_info := {|
+    LOGIC.GS_pre := cpp_preGS Σ thread_info
+  ; LOGIC.GS_ghost := _cpp_ghost
+  |}.
 
   Class cpp_logic {thread_info : biIndex} : Type :=
   { _Σ       : gFunctors
   ; _ghost   : _cpp_ghost
   ; has_cppG : cppG _Σ
   }.
-  Arguments cpp_logic : clear implicits.
+  #[global] Arguments cpp_logic : clear implicits.
   Coercion _Σ : cpp_logic >-> gFunctors.
 
-  #[global] Existing Instance has_cppG.
+  (* Coercing cpp_logic to LOGIC.logic *)
+  #[global] Instance cpp_logic_logic `{Σ : cpp_logic thread_info} : LOGIC.logic thread_info := {|
+    LOGIC._ghost_type := cpp_GS Σ thread_info
+  ; LOGIC._ghost := _ghost
+  ; LOGIC._has_G := has_cppG
+  |}.
+  Coercion cpp_logic_logic : cpp_logic >-> LOGIC.logic.
 
-  Section with_cpp.
-    Context `{cpp_logic ti}.
-
-    Definition mpredI : bi := monPredI ti (iPropI _Σ).
-    Definition mpred := bi_car mpredI.
-
-    (* TODO: seal *)
-    Canonical Structure mpredO : ofe
-      := Ofe mpred (ofe_mixin (monPredO ti (iPropI _Σ))).
-
-    (* We name this, for manual use later when importing [linearity]. *)
-    Lemma mpred_BiAffine : BiAffine mpred.
-    Proof. apply _. Qed.
-  End with_cpp.
-
-  Bind Scope bi_scope with mpred.
+  #[global] Instance cpp_logic_has_inv `{Σ : !cpp_logic thread_info}
+    : invGS Σ := LOGIC.has_inv.
+  #[global] Instance cpp_logic_has_cinv `{Σ : !cpp_logic thread_info}
+    : cinvG Σ := LOGIC.has_cinv.
 End CPP_LOGIC_CLASS_MIXIN.
 
 Module Type CPP_LOGIC_CLASS := CPP_LOGIC_CLASS_BASE <+ CPP_LOGIC_CLASS_MIXIN.
 
 Declare Module LC : CPP_LOGIC_CLASS.
 Export LC.
-
-(**
-To implement higher-order ghost state mentioning [mpred], we
-presuppose [mpred ≈ I -mon> iProp] and use the discrete OFE [I -d>
-iProp Σ] rather than [monPredO]. We cannot use [monPredO] because Iris
-lacks a functor [monPredOF].
-*)
-Definition later_mpredO (Σ : gFunctors) (ti : biIndex) : ofe :=
-  laterO (ti -d> iPropI Σ).
-Definition later_mpredOF (ti : biIndex) : oFunctor :=
-  laterOF (ti -d> idOF).
-Definition later_mpred `{Σ : cpp_logic ti} (P : mpred) :
-    later (ti -d> iPropI Σ) :=
-  Next (monPred_at P).
-
-Section later_mpred.
-  Context `{Σ : cpp_logic ti}.
-
-  #[global] Instance later_mpred_contractive : Contractive later_mpred.
-  Proof.
-    move => n ?? HP. apply: Next_contractive.
-    dist_later_intro. destruct n as [|n]; [lia | by destruct HP].
-  Qed.
-  #[global] Instance later_mpred_ne : NonExpansive later_mpred.
-  Proof. exact: contractive_ne. Qed.
-  #[global] Instance later_mpred_proper : Proper (equiv ==> equiv) later_mpred.
-  Proof. exact: ne_proper. Qed.
-
-  Lemma equivI_later_mpred P Q :
-    later_mpred P ≡ later_mpred Q -|-@{mpredI} |> (P ≡ Q).
-  Proof.
-    rewrite /later_mpred later_equivI.
-    by rewrite discrete_fun_equivI monPred_equivI.
-  Qed.
-End later_mpred.
-#[global] Hint Opaque later_mpred : typeclass_instances.
