theories/lang/base_logic/mpred.v
@@ -1,0 +1,253 @@
+(*
+ * Copyright (c) 2020-2023 BedRock Systems, Inc.
+ * This software is distributed under the terms of the BedRock Open-Source License.
+ * See the LICENSE-BedRock file in the repository root for details.
+ *)
+(**
+This file defines the core [bi] (called [mpred]) that we use for all of our logics.
+It is a [bi] parameterized by:
+1. a thread information (via [monPred]) that allows distinguishing between
+  different implicit contexts, and
+2. a CMRA structure in the style of Iris, i.e. [gFunctors], that allows for
+  higher-order ghost state.
+
+The construction also bakes in the common pattern of allowing to store global
+ghost names directly in the logic rather than needing to pass them separately.
+*)
+
+From iris.base_logic.lib Require Import own cancelable_invariants.
+Require Import iris.bi.monpred.
+
+From bedrock.prelude Require Import base.
+From bedrock.lang Require Import bi.prelude.
+Import ChargeNotation.
+
+Module LOGIC.
+  (** Types of Cmras that a logic requires
+
+  An instance of [GpreS] packages the _types_ of the cmras that a logic's
+  [Σ : gFunctors] should have. By default, we require that any logic's [Σ] should
+  have invariants, i.e. [invGS Σ] and [cinvG Σ].
+
+  For example, a machine logic would have an instance [machineGpreS : GpreS]
+  as follows.
+<<
+  Record machine_preGS {Σ : gFunctors} {thread_info : biIndex} : Type := {
+    machine_pbyte_heapGS : inG Σ (gmapR ...)
+  ; ... (* more Cmras *)
+  ; machine_has_inv : invGS Σ
+  ; machine_has_cinv : cinvG Σ
+  }.
+  #[global] Arguments machine_preGS : clear implicits.
+
+  Definition machineGpreS (Σ : gFunctors) (thread_info : biIndex) : GpreS Σ thread_info := {|
+    preGS := machine_preGS Σ thread_info
+  ; preGS_has_inv := machine_has_inv
+  ; preGS_has_cinv := machine_has_cinv
+  |}.
+>>
+
+  The instance for a NOVA logic [novaGpreS : GpreS] would be as follows.
+<<
+  Record nova_preGS {Σ : gFunctors} {thread_info : biIndex} : Type := {
+    nova_has_machine : machine_preGS Σ thread_info
+  ; ... (* more Cmras *)
+  }.
+  #[global] Arguments nova_preGS : clear implicits.
+
+  Definition novaGpreS (Σ : gFunctors) (thread_info : biIndex) : GpreS Σ thread_info := {|
+    preGS := nova_preGS Σ thread_info
+  ; preGS_has_inv := machine_has_inv ∘ nova_has_machine
+  ; preGS_has_cinv := machine_has_cinv ∘ nova_has_machine
+  |}.
+>>
+
+  The instance for a C++ logic for a C++ abstract machine atop NOVA would build
+  on [novaGpreS] similarly.
+  For a C++ abstract machine that is not built on top of NOVA, its logic would
+  build directly on [machineGpreS].
+  *)
+  Class GpreS {Σ : gFunctors} {thread_info : biIndex} : Type := {
+    preGS : Type
+  ; preGS_has_inv : preGS -> invGS Σ
+  ; preGS_has_cinv : preGS -> cinvG Σ
+  } .
+  Existing Class preGS.
+  #[global] Arguments GpreS : clear implicits.
+  #[global] Hint Mode GpreS - - : typeclass_instances.
+
+  (** Types of cmras and global ghost names that a logic has
+
+  An instance of [GS] packages not only the Cmras, but also the type [GS_ghost]
+  of all global ghost names that a logic relies on.
+<<
+  Record machine_ghost : Type := {
+    machine_pbyte_heap_name : gname
+  ; ... (* more global ghost name types for machine *)
+  }.
+
+  Definition machineGS Σ thread_info : GS Σ thread_info := {|
+    GS_pre := machineGpreS Σ thread_info
+  ; GS_ghost := machine_ghost
+  |}.
+
+  Record nova_ghost : Type := {
+    nova_ghost_has_machine : machine_ghost (* nova_ghost includes machine_ghost *)
+  ; ... (* more global ghost name types for nova *)
+  }.
+
+  Definition novaGS Σ thread_info : GS Σ thread_info := {|
+    GS_pre := novaGpreS Σ thread_info
+  ; GS_ghost := nova_ghost
+  |}.
+>>
+  *)
+  Class GS {Σ : gFunctors} {thread_info : biIndex} : Type := {
+    GS_pre : GpreS Σ thread_info
+  ; GS_ghost : Type
+  }.
+  #[global] Arguments GS : clear implicits.
+  #[global] Hint Mode GS - - : typeclass_instances.
+
+  (** An inclusion relation between ghost types
+
+  [subGS gtype1 gtype2] (tentative notation gtype1 ⊆ gtype2) means that
+  - [subGS_pre]: the cmras of [gtype2] include the cmras of [gtype1]
+  - [subGS_ghost]: the ghost names of [gtype2] include the ghost names of [gtype1]
+
+  This relation captures the fact that one logic is built on top of the other,
+  for example, machineGS ⊆ novaGS ⊆ cppGS means that the C++ logic is built on
+  top of the NOVA logic, which in turn is built on the machine logic.
+  *)
+  Class subGS {Σ : gFunctors} {thread_info : biIndex}
+      (gtype1 gtype2 : GS Σ thread_info) := {
+    subGS_pre : @preGS Σ thread_info gtype2.(GS_pre) -> @preGS Σ thread_info gtype1.(GS_pre)
+  ; subGS_ghost : gtype2.(GS_ghost) -> gtype1.(GS_ghost)
+  }.
+  #[global] Hint Mode subGS - - - - : typeclass_instances.
+
+  (** An instance of a logic
+
+  The instance packages
+  - [_ghost_type : GS _Σ thread_info]: the types of cmras and global ghost names
+    that the logic needs
+  - a gFunctors _Σ that satisfies the requirement of [_ghost_type], i.e. [_has_G]
+    says that _Σ includes the cmras in [_ghost_type.(GS_pre)]
+  - a concrete instance of ghost names [_ghost]
+
+  A logic should have only one such instance, for example there should be only
+  one instance [machine_logic] and one instance [nova_logic].
+  However, we may have multiple C++ logic instances [cpp_logic], each for one
+  C++ abstract machine instance. Each [cpp_logic] would use the same ghost type
+  [cppGS] (GS stands for Ghost Singleton), but would have different concrete
+  ghost names [_ghost].
+  *)
+  Class logic {thread_info : biIndex} : Type :=
+  { _Σ          : gFunctors
+  ; _ghost_type : GS _Σ thread_info
+  ; _ghost      : _ghost_type.(GS_ghost)
+  ; #[global] _has_G :: @preGS _Σ thread_info _ghost_type.(GS_pre)
+  }.
+  #[global] Arguments logic : clear implicits.
+  #[global] Hint Mode logic - : typeclass_instances.
+
+  #[global] Instance has_inv `{!logic thread_info} : invGS _Σ
+    := preGS_has_inv _has_G.
+  #[global] Instance has_cinv `{!logic thread_info} : cinvG _Σ
+    := preGS_has_cinv _has_G.
+
+  (** A logic instance is at least some logic
+
+  The logic instance [Σ] includes [gtype], so it is at least the logic of [gtype].
+  Consequently, any predicates for a logic that only depends on [gtype] can be
+  used in the logic [Σ], that is, they can be embedded into a larger logic.
+
+  To define a predicate that only depends on a concrete GS, we would do the
+  following:
+<<
+  Section pbyte_at.
+    (* pbyte_at only need machine ghosts *)
+    Context `{Σ : logic thread_info} `{!HasGS Σ thread_info (machineGS Σ thread_info)}.
+
+    Definition pbyte_at ... := ...
+  End pbyte_at.
+>>
+  Then, with an instance that [subGS (machineGS Σ thread_info) (novaGS Σ thread_info)],
+  in a context with the nova logic, [pbyte_at] should be usable.
+<<
+  Section nova_logic.
+    Context `{Σ : logic thread_info} `{!HasGS Σ thread_info (novaGS Σ thread_info)}.
+
+    Definitiion vbyte_at ... :=
+      page_mapping ... **
+      pbyte_at ...
+      .
+  End nova_logic.
+>>
+  *)
+  Class HasGS `{Σ : logic thread_info} (gtype : GS _Σ thread_info) := {
+    has_subGS : subGS gtype _ghost_type
+  }.
+  #[global] Hint Mode HasGS - - - : typeclass_instances.
+
+End LOGIC.
+#[global] Coercion LOGIC._Σ : LOGIC.logic >-> gFunctors.
+
+Section mpred.
+  Context `{Σ : !LOGIC.logic thread_info}.
+
+  (* TODO: seal *)
+  Definition mpredI : bi := monPredI thread_info (iPropI Σ).
+  Definition mpred := bi_car mpredI.
+
+  (* TODO: don't make this a Canonical Structure as it depends on LOGIC.logic *)
+  Canonical Structure mpredO : ofe
+    := Ofe mpred (ofe_mixin (monPredO thread_info (iPropI Σ))).
+
+  (* We name this, for manual use later when importing [linearity]. *)
+  Lemma mpred_BiAffine : BiAffine mpred.
+  Proof. apply _. Qed.
+
+  (* HACK: this is to prevent IPM from simplifying [mpred] into [monPred].
+  Sealing mpred is better *)
+  #[global] Instance : BiBUpd mpredI | 0 := monPred_bi_bupd _ _.
+  #[global] Instance : BiFUpd mpredI | 0 := monPred_bi_fupd _ _.
+End mpred.
+
+Bind Scope bi_scope with mpred.
+
+(**
+To implement higher-order ghost state mentioning [mpred], we
+presuppose [mpred ≈ I -mon> iProp] and use the discrete OFE [I -d>
+iProp Σ] rather than [monPredO]. We cannot use [monPredO] because Iris
+lacks a functor [monPredOF].
+*)
+Definition later_mpredO (Σ : gFunctors) (thread_info : biIndex) : ofe :=
+  laterO (thread_info -d> iPropI Σ).
+Definition later_mpredOF (thread_info : biIndex) : oFunctor :=
+  laterOF (thread_info -d> idOF).
+Definition later_mpred `{Σ : !LOGIC.logic thread_info} (P : mpred) :
+    later (thread_info -d> iPropI Σ) :=
+  Next (monPred_at P).
+
+Section later_mpred.
+  Context `{Σ : !LOGIC.logic thread_info}.
+
+  #[global] Instance later_mpred_contractive : Contractive later_mpred.
+  Proof.
+    move => n ?? HP. apply: Next_contractive.
+    dist_later_intro. destruct n as [|n]; [lia | by destruct HP].
+  Qed.
+  #[global] Instance later_mpred_ne : NonExpansive later_mpred.
+  Proof. exact: contractive_ne. Qed.
+  #[global] Instance later_mpred_proper : Proper (equiv ==> equiv) later_mpred.
+  Proof. exact: ne_proper. Qed.
+
+  Lemma equivI_later_mpred P Q :
+    later_mpred P ≡ later_mpred Q -|-@{mpredI} |> (P ≡ Q).
+  Proof.
+    rewrite /later_mpred later_equivI.
+    by rewrite discrete_fun_equivI monPred_equivI.
+  Qed.
+End later_mpred.
+#[global] Hint Opaque later_mpred : typeclass_instances.
